Cslib.lean
@@ -147,6 +147,7 @@ public import Cslib.Logics.Modal.Denotation
 public import Cslib.Logics.Modal.LogicalEquivalence
 public import Cslib.Logics.Propositional.Defs
 public import Cslib.Logics.Propositional.NaturalDeduction.Basic
+public import Cslib.Logics.Propositional.NaturalDeduction.Theory
 public import Cslib.MachineLearning.PACLearning.Defs
 public import Cslib.MachineLearning.PACLearning.VCDimension
 public import Cslib.MachineLearning.PACLearning.VersionSpace
