Cslib/Logics/Propositional/NaturalDeduction/Theory.lean
@@ -1,0 +1,101 @@
+/-
+Copyright (c) 2025 Thomas Waring. All rights reserved.
+Released under Apache 2.0 license as described in the file LICENSE.
+Authors: Thomas Waring
+-/
+module
+
+public import Cslib.Logics.Propositional.NaturalDeduction.Basic
+
+/-! # Results on propositional theories
+
+In this file we prove the expected results that `IPL Atom` is an intuitionistic theory, and
+`CPL Atom` is a classical theory. We provide derived rules for common intuitionistic and classical
+proof patterns.
+-/
+
+@[expose] public section
+
+universe u
+
+namespace Cslib.Logic.PL
+
+open Proposition Theory InferenceSystem DerivableIn Derivation IsIntuitionistic IsClassical
+
+variable {Atom : Type u} [DecidableEq Atom] [Bot Atom] {T : Theory Atom}
+
+namespace Theory
+
+instance instIsIntuitionisticIPL : IsIntuitionistic Atom (IPL Atom) where
+  efq A := ax (efq_mem_ipl A)
+
+/-- Derivation of efq in an arbitrary context. -/
+def IsIntuitionistic.efqCtx [IsIntuitionistic Atom T] (Γ : Ctx Atom) (A : Proposition Atom)
+    : T⇓(Γ ⊢ ⊥ → A) := (efq A : T⇓(⊥ → A)).weakCtx (Finset.empty_subset Γ)
+
+/-- Efq as a derived rule. -/
+def IsIntuitionistic.efqRule [IsIntuitionistic Atom T] (Γ : Ctx Atom) (A : Proposition Atom)
+    (D : T⇓(Γ ⊢ ⊥)) : T⇓(Γ ⊢ A) :=
+  implE (A := ⊥) (efqCtx Γ A) D
+
+/-- Prove any proposition from contradictory hypotheses. -/
+def IsIntuitionistic.contra [IsIntuitionistic Atom T] {Γ : Ctx Atom} (A B : Proposition Atom)
+    (hΓ : A ∈ Γ) (hΓ' : (¬A) ∈ Γ) : T⇓(Γ ⊢ B) :=
+  efqRule Γ B <| implE (ass hΓ') (ass hΓ)
+
+instance instIsClassicalCPL : IsClassical Atom (CPL Atom) where
+  dne A := ax (dne_mem_cpl A)
+
+/-- Proof by contradiction as a derived rule. -/
+def IsClassical.byContra [IsClassical Atom T] {Γ : Ctx Atom} {A : Proposition Atom}
+    (D : T⇓(insert (¬ A) Γ ⊢ ⊥)) : T⇓(Γ ⊢ A) :=
+  implE (A := ¬¬A) ((dne A : T⇓(¬¬A → A)) |>.weakCtx <| Finset.empty_subset ..) D.implI
+
+instance instIsIntuitionisticOfIsClassical [IsClassical Atom T] : IsIntuitionistic Atom T where
+  efq A := implI _ <| byContra <| ass (by grind)
+
+/-- Law of excluded middle in a classical theory. -/
+def IsClassical.lem [IsClassical Atom T] (A : Proposition Atom) : T⇓(A ∨ ¬ A) := by
+  apply byContra
+  apply implE (ass <| Finset.mem_insert_self ..)
+  apply orI₂; apply implI
+  apply implE (A := A ∨ ¬ A) (ass <| by grind)
+  exact orI₁ <| ass <| Finset.mem_insert_self ..
+
+/-- Pierce's law in a classical theory. -/
+def IsClassical.pierce [IsClassical Atom T] (A B : Proposition Atom) : T⇓(((A → B) → A) → A) := by
+  apply implI; apply byContra
+  apply implE (ass <| Finset.mem_insert_self ..)
+  apply implE (A := A → B) (ass <| by grind); apply implI
+  apply contra A B <;> grind
+
+/-- The axiom system consisting of instances of LEM. -/
+def LEM (Atom : Type u) [Bot Atom] : Theory Atom := {A ∨ ¬ A | A : Proposition Atom}
+
+omit [DecidableEq Atom] in
+lemma lem_mem_lem (A : Proposition Atom) : (A ∨ ¬ A) ∈ LEM Atom := ⟨A, rfl⟩
+
+/-- The axiom system consisting of instances of Pierce's law. -/
+def Pierce (Atom : Type u) : Theory Atom :=
+  {((A → B) → A) → A | (A : Proposition Atom) (B : Proposition Atom)}
+
+omit [DecidableEq Atom] [Bot Atom] in
+lemma pierce_mem_pierce (A B : Proposition Atom) : (((A → B) → A) → A) ∈ Pierce Atom := ⟨A, B, rfl⟩
+
+instance instIsClassicalLEM : IsClassical Atom (LEM Atom ∪ IPL Atom : Theory Atom) where
+  dne A := by
+    apply implI
+    apply orE (ax <| Set.mem_union_left _ <| lem_mem_lem A)
+    · exact ass (Finset.mem_insert_self A _)
+    · apply implE (A := ⊥) (ax <| Set.mem_union_right _ (efq_mem_ipl A))
+      apply implE (A := ¬ A) <;> exact ass (by grind)
+
+instance instIsClassicalPierce : IsClassical Atom (Pierce Atom ∪ IPL Atom : Theory Atom) where
+  dne A := by
+    apply implI
+    apply implE (A := (A → ⊥) → A) (ax <| Set.mem_union_left _ <| pierce_mem_pierce A ⊥)
+    apply implI
+    apply implE (A := ⊥) (ax <| Set.mem_union_right _ (efq_mem_ipl A))
+    apply implE (A := ¬ A) <;> exact ass (by grind)
+
+end Cslib.Logic.PL.Theory
